More explicit structure

stlc-naive.v
@@ -261,11 +261,11 @@ Module step.
       star e2 e2' ->
       star (expr.app e1 e2) (expr.app e1 e2').
   Proof.
-    intros e1 e2 e2' Star.
+    intros e1 e2 e2' Star. 
     induction Star.
     - constructor.
     - apply star_trans with (e2 := expr_ast.app e1 e0).
-      + auto.
+      + apply app2. apply H.
       + apply IHStar.
   Qed.
 
@@ -364,12 +364,438 @@ Module has_sem_type.
     eapply E_star; [|now eauto].
 
     eapply step.star_trans'.
-    eapply step.star_app1. now eauto.
-    eapply step.star_trans'.
-    eapply step.star_app2. now eauto.
-    eauto using step.step_l, step.beta, step.star_refl'.
+    - eapply step.star_app1. now eauto.
+    - eapply step.star_trans'.
+      + eapply step.star_app2. now eauto.
+      + eauto using step.step_l, step.beta, step.star_refl'.
   Qed.
 
 End has_sem_type.
 
 End old.
+
+Module new.
+
+Module exprop.
+  Inductive t' :=
+  | abs
+  | app
+  | tt
+  | ff
+  | If
+  .
+  Definition t := t'.
+
+  Definition arity (op : t) : arity.t :=
+    match op with
+    | abs => [1]
+    | app => [0; 0]
+    | tt => []
+    | ff => []
+    | If => [0; 0; 0]
+    end.
+
+  Definition eq_dec : forall x y : t, {x = y} + {x <> y}.
+    decide equality.
+  Defined.
+End exprop.
+
+Module type.
+  Inductive t :=
+  | bool
+  | arrow : t -> t -> t
+  .
+End type.
+
+Module expr_abt := abt.abt exprop.
+
+Module expr_ast.
+  Inductive t :=
+  | var (x : nat) : t
+  | abs : t -> t
+  | app : t -> t -> t
+  | tt : t
+  | ff : t
+  | If : t -> t -> t -> t
+  .
+End expr_ast.
+
+Module expr_basis.
+  Module A := expr_abt.
+
+  Import expr_ast.
+  Definition t := t.
+
+  Fixpoint to_abt (ty : t) : A.t :=
+    match ty with
+    | var n => A.var n
+    | abs e' => A.op exprop.abs [A.bind 1 (to_abt e')]
+    | app e1 e2 => A.op exprop.app [A.bind 0 (to_abt e1); A.bind 0 (to_abt e2)]
+    | tt => A.op exprop.tt []
+    | ff => A.op exprop.ff []
+    | If e1 e2 e3 => A.op exprop.If [A.bind 0 (to_abt e1);
+                                            A.bind 0 (to_abt e2);
+                                            A.bind 0 (to_abt e3)]
+    end.
+
+  Fixpoint of_abt (a : A.t) : t :=
+    match a with
+    | A.var n => var n
+    | A.op exprop.abs [A.bind 1 a'] => abs (of_abt a')
+    | A.op exprop.app [A.bind 0 a1; A.bind 0 a2] => app (of_abt a1) (of_abt a2)
+    | A.op exprop.tt [] => tt
+    | A.op exprop.ff [] => ff
+    | A.op exprop.If [A.bind 0 a1; A.bind 0 a2; A.bind 0 a3] =>
+      If (of_abt a1) (of_abt a2) (of_abt a3)
+    | _ => var 0 (* bogus *)
+    end.
+
+  Fixpoint shift c d (e : t) : t :=
+    match e with
+    | var x => var (if x <? c then x else x + d)
+    | abs e' => abs (shift (S c) d e')
+    | app e1 e2 => app (shift c d e1) (shift c d e2)
+    | tt => tt
+    | ff => ff
+    | If e1 e2 e3 => If (shift c d e1) (shift c d e2) (shift c d e3)
+    end.
+
+  Fixpoint subst rho e :=
+    match e with
+    | var x => match nth_error rho x with
+                  | Some e' => e'
+                  | None => e
+                  end
+    | abs e' => abs (subst (var 0 :: map (shift 0 1) rho) e')
+    | app e1 e2 => app (subst rho e1) (subst rho e2)
+    | tt => tt
+    | ff => ff
+    | If e1 e2 e3 => If (subst rho e1) (subst rho e2) (subst rho e3)
+    end.
+
+  Fixpoint wf n e :=
+    match e with
+    | var x => x < n
+    | abs e' => wf (S n) e'
+    | app e1 e2 => wf n e1 /\ wf n e2
+    | tt => True
+    | ff => True
+    | If e1 e2 e3 => wf n e1 /\ wf n e2 /\ wf n e3
+    end.
+
+  Fixpoint identity_subst (n : nat) : list t :=
+    match n with
+    | 0 => []
+    | S n => var 0 :: map (shift 0 1) (identity_subst n)
+    end.
+
+  Lemma ws_to_abt : forall e, A.ws (to_abt e).
+  Proof. A.basis_util.prove_ws_to_abt. Qed.
+
+  Lemma of_to_abt : forall e, of_abt (to_abt e) = e.
+  Proof. A.basis_util.prove_of_to_abt. Qed.
+
+  Lemma to_of_abt : forall a, A.ws a -> to_abt (of_abt a) = a.
+  Proof. A.basis_util.prove_to_of_abt to_abt of_abt. Qed.
+
+  Lemma shift_to_abt_comm : forall e c d, to_abt (shift c d e) = A.shift c d (to_abt e).
+  Proof. A.basis_util.prove_shift_to_abt_comm. Qed.
+
+  Lemma map_shift_to_abt_comm :
+    forall c d rho, map to_abt (map (shift c d) rho) = map (A.shift c d) (map to_abt rho).
+  Proof. A.basis_util.prove_map_shift_to_abt_comm shift_to_abt_comm. Qed.
+
+  Lemma subst_to_abt_comm : forall e rho,
+      to_abt (subst rho e) = A.subst (map to_abt rho) (to_abt e).
+  Proof. A.basis_util.prove_subst_to_abt_comm t map_shift_to_abt_comm. Qed.
+
+  Lemma wf_to_abt : forall e n, wf n e <-> A.wf n (to_abt e).
+  Proof. A.basis_util.prove_wf_to_abt. Qed.
+
+  Lemma identity_subst_to_abt_comm :
+    forall n, List.map to_abt (identity_subst n) = A.identity_subst n.
+  Proof. A.basis_util.prove_identity_subst_to_abt_comm map_shift_to_abt_comm. Qed.
+
+  Definition var := var.
+  Arguments var /.
+  Lemma var_to_abt : forall n, to_abt (var n) = A.var n.
+  Proof. reflexivity. Qed.
+End expr_basis.
+
+Module expr.
+  Include abt.abt_util expr_basis.
+  Notation abs := expr_ast.abs.
+  Notation app := expr_ast.app.
+  Notation tt := expr_ast.tt.
+  Notation ff := expr_ast.ff.
+  Notation If := expr_ast.If.
+End expr.
+
+Module value.
+  Inductive t : expr.t -> Prop :=
+  | tt : t expr.tt
+  | ff : t expr.ff
+  | abs : forall e, t (expr.abs e)
+  .
+End value.
+
+Module step.
+  Inductive t : expr.t -> expr.t -> Prop :=
+  | beta : forall e1 e2,
+      value.t e2 ->
+      t (expr.app (expr.abs e1) e2)
+        (expr.subst [e2] e1)
+  | app1  : forall e1 e1' e2,
+      t e1 e1' ->
+      t (expr.app e1 e2) (expr.app e1' e2)
+  | app2  : forall e1 e2 e2',
+      value.t e1 ->
+      t e2 e2' ->
+      t (expr.app e1 e2) (expr.app e1 e2')
+  | IfT : forall e2 e3,
+      t (expr.If expr.tt e2 e3) e2
+  | IfF : forall e2 e3,
+      t (expr.If expr.ff e2 e3) e3
+  | If : forall e1 e1' e2 e3,
+      t e1 e1' ->
+      t (expr.If e1 e2 e3) (expr.If e1' e2 e3)
+  .
+  Hint Constructors t.
+
+  (* 
+   * Inlining star explicitly as an application of clos_refl_trans_n1 to
+   * make it clearer what these proofs are doing for patching purposes
+   *)
+  Inductive star (e1 : expr.t) : expr.t -> Prop :=
+    | star_refl : star e1 e1
+    | star_trans (e2 e3 : expr.t) :
+        t e2 e3 -> star e1 e2 -> star e1 e3.
+
+  Inductive star_l (e1 : expr.t) : expr.t -> Prop :=
+    | star_step_l (e2 : expr.t) : t e1 e2 -> star_l e1 e2
+    | star_refl_l : star_l e1 e1
+    | star_trans_l (e2 e3 : expr.t) :
+        star_l e1 e2 -> star_l e2 e3 -> star_l e1 e3.
+
+  Lemma star_l_star : forall e1 e2,
+    star_l e1 e2 -> star e1 e2.
+  Proof.
+    intros. induction H.
+    - apply star_trans with (e2 := e1).
+      + auto.
+      + constructor.
+    - apply star_refl.
+    - elim IHstar_l2; auto.
+      intros.
+      eapply star_trans; eauto.
+  Qed.
+
+  Lemma star_star_l : forall e1 e2,
+    star e1 e2 -> star_l e1 e2.
+  Proof.
+    intros. induction H.
+    - apply star_refl_l.
+    - apply star_trans_l with (e2 := e2).
+      + auto.
+      + apply star_step_l. auto.
+  Qed. 
+
+  Lemma step_l :
+    forall e1 e2 e3,
+      t e1 e2 ->
+      star e2 e3 ->
+      star e1 e3.
+  Proof.
+    intros e1 e2 e3 S Star.
+    apply star_l_star.
+    apply star_star_l in Star.
+    eapply star_trans_l; eauto using star_step_l.
+  Qed.
+
+  Lemma star_app1 :
+    forall e1 e1' e2,
+      star e1 e1' ->
+      star (expr.app e1 e2) (expr.app e1' e2).
+  Proof.
+    intros e1 e1' e2 Star.
+    induction Star.
+    - constructor.
+    - apply star_trans with (e2 := expr.app e0 e2).
+      + auto.
+      + apply IHStar.
+  Qed.
+
+  Lemma star_app2 :
+    forall e1 e2 e2',
+      value.t e1 ->
+      star e2 e2' ->
+      star (expr.app e1 e2) (expr.app e1 e2').
+  Proof.
+    intros e1 e2 e2' Val1 Star.
+    induction Star.
+    - constructor.
+    - apply star_trans with (e2 := expr_ast.app e1 e0).
+      + apply app2.
+        * apply Val1.
+        * apply H.
+      + apply IHStar.
+  Qed.
+
+  Lemma star_trans' :
+    forall e1 e2 e3,
+      star e1 e2 ->
+      star e2 e3 ->
+      star e1 e3.
+  Proof.
+    intros e1 e2 e3 S1 S2.
+    apply star_star_l in S1.
+    apply star_star_l in S2.
+    apply star_l_star.
+    eauto using star_trans_l.
+  Qed.
+
+  Lemma star_refl' :
+    forall e,
+      star e e.
+  Proof.
+    constructor.
+  Qed.
+
+End step.
+
+Module terminating.
+  Definition t (P : expr.t -> Prop) (e : expr.t) :=
+    exists v,
+      step.star e v /\
+      value.t v /\
+      P v
+  .
+End terminating.
+
+Fixpoint V ty e :=
+  match ty with
+    | type.bool => e = expr.tt \/ e = expr.ff
+    | type.arrow ty1 ty2 =>
+      expr.wf 0 e /\
+      exists body,
+          e = expr.abs body /\
+          forall e2,
+            V ty1 e2 ->
+            terminating.t (V ty2) (expr.subst [e2] body)
+  end.
+
+Lemma E_step :
+  forall ty e e',
+    step.t e e' ->
+    terminating.t (V ty) e' ->
+    terminating.t (V ty) e.
+Proof.
+  intros ty e e' S HE.
+  revert ty HE.
+  induction S; intros ty0 [v [Star [Val HV]]]; exists v; intuition.
+  all: eapply step.step_l; eauto.
+Qed.
+
+Lemma E_star :
+  forall ty e e',
+    step.star e e' ->
+    terminating.t (V ty) e' ->
+    terminating.t (V ty) e.
+Proof.
+  intros ty e e' Star HE.
+  revert ty HE.
+  now induction Star; eauto using E_step.
+Qed.
+
+Module has_sem_type.
+  Definition t G e ty :=
+    expr.wf (length G) e /\
+    forall vs,
+      Forall2 V G vs ->
+      terminating.t (V ty) (expr.subst vs e).
+
+  Lemma app :
+    forall G e1 e2 ty1 ty2,
+      t G e1 (type.arrow ty1 ty2) ->
+      t G e2 ty1 ->
+      t G (expr.app e1 e2) ty2.
+  Proof.
+    intros G e1 e2 ty1 ty2.
+    intros [WF1 HT1].
+    intros [WF2 HT2].
+    split; [now cbn; auto|].
+    intros vs F.
+
+    cbn [expr.subst].
+    specialize (HT1 vs F).
+    specialize (HT2 vs F).
+    destruct HT1 as [v1 [Star1 [Val1 V1]]].
+    destruct HT2 as [v2 [Star2 [Val2 V2]]].
+    destruct V1 as [WFv1 [body1 [? H1]]].
+    subst v1.
+    eapply E_star; [|now eauto].
+
+    eapply step.star_trans'.
+    - eapply step.star_app1. now eauto.
+    - eapply step.star_trans'.
+      + eapply step.star_app2.
+        * apply Val1. 
+        * now eauto.
+      + eauto using step.step_l, step.beta, step.star_refl'.
+  Qed.
+
+End has_sem_type.
+
+End new.
+
+Print old.step.star_app2.
+
+(*
+star_app2 (e1 e2 e2' : expr.t) (Star : star e2 e2') :=
+  star_ind
+    e2
+    (fun e2'0 : expr.t => star (expr_ast.app e1 e2) (expr_ast.app e1 e2'0))
+    (star_refl (expr_ast.app e1 e2))
+    (fun (e0 e3 : expr.t) (H : t e0 e3) (_ : star e2 e0)
+         (IHStar : star (expr_ast.app e1 e2) (expr_ast.app e1 e0)) =>
+      star_trans
+        (expr_ast.app e1 e2)
+        (expr_ast.app e1 e0)
+        (expr_ast.app e1 e3)
+        (app2 e1 e0 e3 H)
+        IHStar) 
+    e2'
+    Star
+: forall (e1 e2 e2' : expr.t),
+    star e2 e2' -> star (expr_ast.app e1 e2) (expr_ast.app e1 e2')
+*)
+
+Print new.step.star_app2.
+
+(*
+star_app2 (e1 e2 e2' : expr.t) (Val1 : value.t e1) (Star : step.star e2 e2') :=
+  star_ind
+    e2
+    (fun e2'0 : expr.t => star (expr_ast.app e1 e2) (expr_ast.app e1 e2'0))
+    (star_refl (expr_ast.app e1 e2))
+    (fun (e0 e3 : expr.t) (H : t e0 e3) (_ : star e2 e0)
+         (IHStar : star (expr_ast.app e1 e2) (expr_ast.app e1 e0)) =>
+      star_trans
+        (expr_ast.app e1 e2)
+        (expr_ast.app e1 e0)
+        (expr_ast.app e1 e3)
+        (app2 e1 e0 e3 Val1 H)
+        IHStar)
+    e2'
+    Star
+: forall (e1 e2 e2' : expr.t),
+       value.t e1 ->
+       star e2 e2' -> star (expr_ast.app e1 e2) (expr_ast.app e1 e2')
+*)
+
+(*
+ * Without revert and with explicit structure, the patch becomes clearer.
+ * But note that this doesn't tell us generally how to repair an app2.
+ * This tells us how to repair an app2 inside of a star_ind.
+ *)
+
